lean/Ttac.lean
@@ -14,3 +14,4 @@ import Ttac.VcSound
 import Ttac.VcPrefix
 import Ttac.VcCfgPath
 import Ttac.VcDenot
+import Ttac.VcWeaken
